Start using big_opLZ lemmas.

rocq-osiris/theories/program_logic/rules/array_rules.v
@@ -2,7 +2,7 @@ From iris Require Import gen_heap proofmode.proofmode.
 From osiris Require Import lang.
 From osiris.program_logic Require Import ewp.
 From osiris.program_logic.rules Require Import impure_rules stop_rules.
-From osiris.logic Require Import list_z.
+From osiris.logic Require Import list_z big_opLZ.
 
 Definition array : Type := list loc.
 
@@ -21,108 +21,41 @@ Section array_resources.
 
   Definition isSlice `{Encode A} dq (ls : array) (i : Z) (xs : list A) : iProp Σ :=
     ⌜0 ≤ i ∧ i + length xs ≤ length ls⌝ ∗
-    [∗ list] l;x ∈ take (length xs) (drop i ls); xs, pointsto l dq (V #x).
+    [∗ listZ] l;x ∈ seg i (i + length xs) ls; xs, pointsto l dq (V #x).
 
   Arguments isSlice {_ _} dq a i xs : rename.
 
-  Lemma leq_length {A} (i : Z) (l : list A) :
-    0 ≤ i ≤ length l →
-    ∃ li lrest, l = li ++ lrest ∧ i = length li.
+  Lemma split_Slice `{Encode A} (j : Z) dq a i (xs ys zs : list A) :
+    xs = ys ++ zs →
+    j = i + length ys →
+    isSlice dq a i xs ⊣⊢ (isSlice dq a i ys ∗ isSlice dq a j zs).
   Proof.
-    intros Hpos.
-    exists (take i l), (drop i l).
-    split. by rewrite take_drop. rewrite length_take.
-    lia.
-  Qed.
+    length_nonneg ys; length_nonneg zs; length_nonneg a.
+    intros -> ->.
+    iStartProof; iSplit; iIntros "Hslice".
+    - unfold isSlice. length.
+      iDestruct "Hslice" as "([%Hpos %Hlen] & Hseg)".
+      rewrite -(assoc bi_sep).
+      iSplitR. { iPureIntro; length_nonneg zs; lia. }
+      rewrite (comm bi_sep) -(assoc bi_sep).
+      iSplitR. { iPureIntro; length_nonneg ys; lia. }
+      rewrite (comm bi_sep). iApply big_sepLZ2_app_inv; first (length; lia).
+      rewrite (split_seg (i + length ys)); try lia.
+      rewrite (assoc Z.add). iFrame.
 
-  Lemma eq_length {A} (i j : Z) (l : list A) :
-    0 ≤ i ∧ 0 ≤ j →
-    i + j = length l →
-    ∃ li lj, l = li ++ lj ∧ i = length li ∧ j = length lj.
-  Proof.
-    intros Hpos Heq.
-    exists (take i l), (drop i l).
-    split. by rewrite take_drop. rewrite length_take length_drop. lia.
+    - iDestruct "Hslice" as "(Hslice1 & Hslice2)".
+      iDestruct "Hslice1" as "([%Hpos %Hlen] & Hslice1)".
+      iDestruct "Hslice2" as "([%Hpos' %Hlen'] & Hslice2)".
+      iSplit.
+      { iPureIntro; length; lia. }
+      iPoseProof (big_sepLZ2_app with "Hslice1 Hslice2") as "Hslice".
+      rewrite -(split_seg (i + length ys)); try lia.
+      length; rewrite (assoc Z.add).
+      iApply "Hslice".
   Qed.
-
-  Local Lemma decompose_list {A} (i j k : Z) (ls : list A) :
-    (0 ≤ i ∧ 0 ≤ j ∧ 0 ≤ k) →
-    (i + j + k ≤ length ls) →
-    ∃ li lys lzs lextra,
-      ls = li ++ lys ++ lzs ++ lextra ∧
-      i = length li ∧ j = length lys ∧ k = length lzs.
-  Proof.
-    intros Hpos constraint.
-    assert (0 ≤ i + j + k ∧ i + j + k ≤ length ls) as Hpos' by lia.
-    apply leq_length in Hpos' as (l' & lextra & -> & Hlen).
-    apply eq_length in Hlen as (l1 & l2 & -> & Hlen1 & Hlen2); last lia.
-    apply eq_length in Hlen1 as (l1' & l2' & -> & Hlen1' & Hlen2'); last lia.
-    exists l1', l2', l2, lextra.
-    rewrite !app_assoc. auto.
-  Qed.
-
-  Local Lemma cut_out_slice {A} (i j : Z) (ls : list A) :
-    (0 ≤ i ∧ 0 ≤ j) →
-    (i + j ≤ length ls) →
-    ∃ li slice lextra,
-      ls = li ++ slice ++ lextra ∧
-      i = length li ∧ j = length slice.
-  Proof.
-    intros Hpos constraint.
-    assert (0 ≤ i + j ∧ i + j ≤ length ls) as Hpos' by lia.
-    apply leq_length in Hpos' as (l' & lextra & -> & Hlen).
-    apply eq_length in Hlen as (l1 & l2 & -> & Hlen1 & Hlen2); last lia.
-    exists l1, l2, lextra. rewrite app_assoc. auto.
-  Qed.
-
-   Lemma split_Slice `{Encode A} (j : Z) dq a i (xs ys zs : list A) :
-     xs = ys ++ zs →
-     j = i + length ys →
-     isSlice dq a i xs ⊣⊢ (isSlice dq a i ys ∗ isSlice dq a j zs).
-   Proof.
-     intros -> ->.
-     iStartProof; iSplit; iIntros "Hslice".
-     - iDestruct "Hslice" as "([%Hpos %Hlen] & Hslice)".
-       rewrite length_app in Hlen.
-       replace (i + (length ys + length zs))
-         with (i + length ys + length zs) in Hlen by lia.
-       (* Decompose [ls] into [li ++ lys ++ lzs ++ lextra]. *)
-       assert (0 ≤ length ys)%Z by apply (length_nonneg).
-       assert (0 ≤ length zs)%Z by apply (length_nonneg).
-       assert (0 ≤ i ∧ 0 ≤ length ys ∧ 0 ≤ length zs) as Hpos' by lia.
-       destruct (decompose_list _ _ _ a Hpos' Hlen)
-         as (li & lys & lzs & lextra & -> & Hlen1 & Hlen2 & Hlen3).
-       rewrite /sub /seg.
-       drop. take.
-       iPoseProof (big_sepL2_app_inv with "Hslice") as "[Hslice1 Hslice2]".
-       { rewrite /length in Hlen2. lia. }
-       iSplitL "Hslice1".
-       + iSplit.
-         { iPureIntro. rewrite !length_app in Hlen |-*. lia. }
-         rewrite /sub /seg.
-         drop. take.
-         iApply "Hslice1".
-       + iSplit.
-         { iPureIntro. rewrite !length_app in Hlen |- *. lia. }
-         rewrite /sub /seg.
-         drop. take.
-         iApply "Hslice2".
-     - iDestruct "Hslice" as "(Hslice1 & Hslice2)".
-       iDestruct "Hslice1" as "([%Hpos %Hlen] & Hslice1)".
-       iDestruct "Hslice2" as "([%Hpos' %Hlen'] & Hslice2)".
-       iSplit.
-       { iPureIntro. rewrite length_app. lia. }
-       (* Decompose [ls] into [li ++ lys ++ lzs ++ lextra]. *)
-       length_nonneg ys. length_nonneg zs.
-       assert (0 ≤ i ∧ 0 ≤ length ys ∧ 0 ≤ length zs) as Hpos'' by lia.
-       destruct (decompose_list _ _ _ a Hpos'' Hlen')
-         as (li & lys & lzs & lextra & -> & Hlen1 & Hlen2 & Hlen3).
-       drop. take.
-       iApply (big_sepL2_app with "Hslice1 Hslice2").
-   Qed.
 
    Definition isArrayCell `{Encode A} dq (a : array) (i : nat) (x : A) : iProp Σ :=
-     isSlice dq a i [x].
+     isSlice dq a i (singleton x).
 
    Definition ownArray `{Encode A} (a : array) (xs : list A) : iProp Σ :=
      isArray a (length xs) ∗ isSlice (DfracOwn 1) a 0 xs.
@@ -152,9 +85,9 @@ Section array_resources.
 
    Lemma imp_EArrayLit `{Encode A} {ζ} (Φs : list (A → iProp Σ)) es :
      ⌜length Φs = length es ∧ length es ≤ max_array⌝ -∗
-     imp evals η es @ E <|Ψ|> ⟨⟨ ζ ⟩⟩ {{ λ xs, [∗ list] x;Φ ∈ xs;Φs, Φ x }} -∗
+     imp evals η es @ E <|Ψ|> ⟨⟨ ζ ⟩⟩ {{ λ xs, [∗ listZ] x;Φ ∈ xs;Φs, Φ x }} -∗
      imp eval η (EArrayLit es) @ E <|Ψ|> ⟨⟨ ζ ⟩⟩
-       {{ λ a, ∃ xs, ownArray a xs ∗ [∗ list] x;Φ ∈ xs;Φs, Φ x }}.
+       {{ λ a, ∃ xs, ownArray a xs ∗ [∗ listZ] x;Φ ∈ xs;Φs, Φ x }}.
    Proof.
      iIntros "[%Hleneq %Hlenbound] He". simpl_eval.
      iApply (imp_bind (A1:=list A) with "He").
@@ -163,20 +96,17 @@ Section array_resources.
      iIntros "!>" (ls) "Hls".
      rewrite /continue /=.
      iApply (imp_ret _ ls); first encode.
-     iPoseProof (big_sepL2_length with "Hls") as "%Hlenls".
-     assert (length ls = length xs).
-     { rewrite length_map in Hlenls. rewrite /length. lia. }
-     iPoseProof (big_sepL2_length with "HΦs") as "%Hlenxs".
-     assert (length xs = length Φs).
-     { rewrite /length. apply inj_eq. assumption. }
-     iExists xs.
-     iSplitL "Hls".
-     { iSplit. iPureIntro; length_nonneg es; lia.
-       rewrite /isSlice. iSplit; first (iPureIntro; lia).
-       drop. take.
-       iApply (big_sepL2_fmap_r encode.encode (λ _ l v, l ↦ v)%I).
-       iApply "Hls". }
+     iPoseProof (big_sepLZ2_length with "Hls") as "%Hlenls".
+     rewrite length_map in Hlenls.
+     iPoseProof (big_sepLZ2_length with "HΦs") as "%Hlenxs".
      iFrame.
+     iSplitR.
+     - iPureIntro.
+       length_nonneg es; rewrite Hlenls Hlenxs Hleneq; lia.
+     - iSplit. { iPureIntro; lia. }
+       rewrite -Hlenls. seg.
+       iApply (big_sepLZ2_fmap_r encode.encode (λ _ l v, l ↦ v)%I).
+       iApply "Hls".
    Qed.
 
    Lemma imp_EArrayEmpty `{Encode A} {ζ} :
@@ -187,12 +117,10 @@ Section array_resources.
      - iApply (imp_EArrayLit (@nil (A → _))  []).
        iPureIntro; length; split; auto.
        pose proof (max_array_positive). lia.
-       simpl_evals. iApply imp_ret; [ encode | auto ].
+       simpl_evals. iApply imp_ret; first encode.
+       by iApply big_sepLZ2_nil.
      - iIntros (a) "(%xs & HownArr & Hxs)".
-       iPoseProof (big_sepL2_length with "Hxs") as "%Hlen".
-       assert (xs = []) as ->.
-       { apply list.nil_length_inv, Hlen. }
-       iApply "HownArr".
+       by iPoseProof (big_sepLZ2_nil_inv_r with "Hxs") as "->".
    Qed.
 
    Lemma imp_EArrayLength {ζ} (n : Z) e :
@@ -206,20 +134,6 @@ Section array_resources.
      change (♯ls) with ls.
      iApply (imp_ret (VInt (repr (length ls))) (length ls)%Z). encode.
      iPureIntro. lia.
-   Qed.
-
-   Lemma list_elem_of_split_length {A : Type} (l : list A) (i : Z) (x : A) :
-     l !! i = Some x → ∃ l1 l2 : list A, l = l1 ++ x :: l2 ∧ i = length l1.
-   Proof.
-     intros Hlookup.
-     pose proof (list_z.lookup_lt_Some l i x Hlookup) as Hvalid.
-     rewrite /lookup /listz_lookup in Hlookup.
-     rewrite /list_z.length in Hvalid.
-     rewrite (decide_False) in Hlookup; last lia.
-     pose proof (list_elem_of_split_length _ _ _ Hlookup)
-       as (l1 & l2 & -> & Hlength).
-     eexists l1, l2; split; [ reflexivity | ].
-     rewrite /length. lia.
    Qed.
 
    Lemma imp_EArrayMake `{Encode A} {ζ} {e1 e2} (n : Z) (Φ : A → iProp Σ) :
@@ -239,26 +153,58 @@ Section array_resources.
      - iIntros (e) "Hζ !>".
        iApply (imp_throw with "Hζ").
      - iIntros (? a) "-> Hφ !> /=".
-       rewrite bind_ret.
-       rewrite signed_repr; last representable.
+       rewrite bind_ret signed_repr; last representable.
        case_decide; last contradiction.
        iApply imp_allocn.
        iIntros "!>" (ls) "Hpts".
-       iPoseProof (big_sepL2_length with "Hpts") as "%Hlen'".
-       assert (length ls = n) as Hlen.
-       { pose proof (length_replicate n #a) as Hlen_z.
-         rewrite /length in Hlen_z |- *. lia. }
+       iPoseProof (big_sepLZ2_length with "Hpts") as "%Hlen'".
+       rewrite length_replicate in Hlen'.
        rewrite /continue /=.
-       iApply imp_ret. encode.
+       iApply imp_ret; first encode.
        iFrame.
-       iSplitR.
-       { iPureIntro. rewrite length_replicate. lia. }
-       iSplit.
-       { iPureIntro; rewrite length_replicate. lia. }
-       drop. take.
-       iApply (big_sepL2_fmap_r encode.encode (λ _ l v, l ↦ v)%I).
-       rewrite fmap_replicate.
+       iSplitR. { iPureIntro; length; lia. }
+       iSplit. { iPureIntro; length; lia. }
+       seg.
+       rewrite -fmap_replicate big_sepLZ2_fmap_r.
        iApply "Hpts".
+   Qed.
+
+   Global Instance inhabited_loc : Inhabited loc.
+   Proof.
+     do 2 constructor. apply Z.inhabited.(inhabitant).
+   Qed.
+
+   Lemma big_sepLZ2_lookup_seg_acc `{Inhabited A, Inhabited B} k i j (xs : list A) (ys : list B) (Φ : Z → A → B → iProp Σ) :
+     valid_seg i j xs →
+     i ≤ k < j →
+     ([∗ listZ] k↦l; x ∈ seg i j xs; ys, Φ k l x) -∗
+     Φ (k - i) (xs !!! k) (ys !!! (k - i)) ∗
+     (Φ (k - i) (xs !!! k) (ys !!! (k - i)) -∗ [∗ listZ] k↦l; x ∈ seg i j xs; ys, Φ k l x).
+   Proof.
+     iIntros (Hvalid Hlek) "Hseg".
+     iPoseProof (big_sepLZ2_length with "Hseg") as "%Hlen".
+     iApply (big_sepLZ2_lookup_acc _ _ _ (k - i) with "Hseg"); lookup.
+     - replace (i + (k - i)) with k by lia.
+       apply list_lookup_lookup_total_valid. lia.
+     - apply list_lookup_lookup_total_valid.
+       revert Hlen. length. lia.
+   Qed.
+
+   Lemma big_sepLZ2_insert_seg_acc `{Inhabited A, Inhabited B} k i j (xs : list A) (ys : list B) (Φ : Z → A → B → iProp Σ) :
+     valid_seg i j xs →
+     i ≤ k < j →
+     ([∗ listZ] k↦l; x ∈ seg i j xs; ys, Φ k l x) -∗
+     Φ (k - i) (xs !!! k) (ys !!! (k - i)) ∗
+     (∀ x y, Φ (k - i) x y -∗ [∗ listZ] n↦l; x ∈seg i j (<[k:=x]>xs); <[k-i:=y]>ys, Φ n l x).
+   Proof.
+     iIntros (Hvalid Hlek) "Hseg".
+     iPoseProof (big_sepLZ2_length with "Hseg") as "%Hlen".
+     setoid_rewrite seg_insert_inside; last lia.
+     iApply (big_sepLZ2_insert_acc _ _ _ (k - i) with "Hseg"); lookup.
+     - replace (i + (k - i)) with k by lia.
+       apply list_lookup_lookup_total_valid. lia.
+     - apply list_lookup_lookup_total_valid.
+       revert Hlen. length. lia.
    Qed.
 
    Lemma imp_EArrayGet2 `{Encode A, Inhabited A} {Φ : A → iProp Σ} {ζ} (Φ1 : array → iProp Σ) (Φ2 : Z → iProp Σ) e1 e2 :
@@ -266,9 +212,9 @@ Section array_resources.
      imp eval η e2 @ E <|Ψ|> ⟨⟨ ζ ⟩⟩ {{ λ i, Φ2 i }} -∗
      (∀ a i, Φ1 a -∗ Φ2 i -∗
              ∃ n, isArray a n ∗
-             ∃ dq j xs (x : A),
-               ▷ (⌜j ≤ i⌝ ∗ ⌜i - j < length xs⌝ ∗ isSlice dq a j xs ∗ ⌜xs !!! (i - j) = x⌝) ∗
-               ▷ (isSlice dq a j xs -∗ Φ x)) -∗
+             ∃ dq j xs,
+               ▷ (⌜j ≤ i⌝ ∗ ⌜i - j < length xs⌝ ∗ isSlice dq a j xs) ∗
+               ▷ (isSlice dq a j xs -∗ Φ (xs !!! (i - j)))) -∗
      imp eval η (EArrayGet e1 e2) @ E <|Ψ|> ⟨⟨ ζ ⟩⟩ {{ Φ }}.
    Proof.
      iIntros "He1 He2 P". simpl_eval.
@@ -282,66 +228,22 @@ Section array_resources.
        iApply (imp_throw with "Hζ"). }
      iIntros (ls i) "HΦ1 HΦ2".
      iDestruct ("P" with "HΦ1 HΦ2")
-       as "(%n & #Harr & %dq & %j & %xs & %x & P)".
+       as "(%n & #Harr & %dq & %j & %xs & P)".
      rewrite /continue /= bind_ret.
      iNext.
-     iDestruct "P" as "((%Hle & %Hlt & Hslice & %Htotal_lookup) & P)".
-
+     iDestruct "P" as "((%Hle & %Hlt & Hslice) & P)".
      iDestruct "Harr" as "(%Hlen' & %Hbound)".
      iDestruct "Hslice" as "(%Hlen & Hslice)".
-
-     (* Decompose [ls] into [lj ++ slice ++ _]. *)
-     pose proof (cut_out_slice j (length xs) ls ltac:(lia) ltac:(lia))
-       as (lj & slice & lextra & Hls & Hj & Hslice).
-     (* Turn [take _ (drop _ ls)] into [slice]. *)
-     rewrite Hj {1}Hls. drop.
-     rewrite Hslice. take.
-
-     assert (¬ (i - j < 0)) as Heqf by lia.
-
-     rewrite (signed_repr i); last representable.
-     assert (list_z.valid (i - j) xs) as Hvalid by lia.
-     pose proof (list_lookup_lookup_total_valid xs (i - j) Hvalid) as Hlookup.
-
-     (* [Decompose [xs] intl [xk ++ x :: _]. *)
-     pose proof (list_elem_of_split_length xs (i - j) _ Hlookup)
-       as (xk & xrest & Hxs & Hxk).
-     rewrite {1}Hxs.
-
-     (* Inversions on [Hslice] gives us that
-        [slice] = [slicek ++ l :: _]. *)
-     iDestruct (big_sepL2_app_inv_r with "Hslice")
-       as "(%slicek & %slice' & -> & Hslice1 & Hslice2)".
-     iDestruct (big_sepL2_cons_inv_r with "Hslice2") as
-       "(%l & %slicerest & -> & Hl & Hslice2)".
-
-     (* We can now prove that [ls !! i] = [Some l]. *)
-     rewrite {2}Hls lookup_app_r; last lia.
-     rewrite <- Hj.
-     rewrite <- app_assoc. iPoseProof (big_sepL2_length with "Hslice1") as "%Hleneq".
-     assert (length ls = j + length slicek + 1 + length slicerest + length lextra).
-     { rewrite Hls. rewrite !length_app. rewrite length_cons. lia. }
-     assert (length slicek = length xk) by (rewrite /length; lia).
-     rewrite lookup_app_r; last lia.
-     assert (i - j - length slicek = 0) as -> by lia.
-     rewrite <- app_comm_cons.
-     rewrite lookup_cons_eq_0.
-
+     rewrite signed_repr; last representable.
+     rewrite list_lookup_lookup_total_valid; last lia.
+     iPoseProof (big_sepLZ2_lookup_seg_acc i with "Hslice")
+       as "(Hl & Hslice)"; try lia.
      iApply (imp_load with "Hl").
-     rewrite /continue; iIntros "!> Hl /=".
+     iIntros "!> Hl".
      iApply imp_ret; first encode.
-     rewrite Htotal_lookup. iApply "P".
-     iCombine ("Hl Hslice2") as "Hslice2".
-     iPoseProof (big_sepL2_cons (λ _ l' x', pointsto l' dq (V #x')) with "Hslice2") as "Hslice2".
-     iPoseProof (big_sepL2_app with "Hslice1 Hslice2") as "Hslice".
-     iSplit.
-     { iPureIntro. lia. }
-     rewrite {1}Hls.
-     rewrite Hj. rewrite drop_app drop_all Z.sub_diag drop_none. simpl.
-     assert (length xs = length (slicek ++ l :: slicerest)) as -> by lia.
-     rewrite take_app_length.
-     rewrite Hxs. rewrite Htotal_lookup.
-     iApply "Hslice".
+     iApply "P".
+     iSplit. { iPureIntro; apply Hlen. }
+     iApply ("Hslice" with "Hl").
    Qed.
 
    Lemma imp_EArrayGet `{Encode A, Inhabited A} {ζ} a (n : Z) (i j : Z) dq (xs : list A) x e1 e2 :
@@ -363,10 +265,10 @@ Section array_resources.
      iIntros (? ?) "-> ->".
      iFrame "#".
      iFrame "%". iFrame.
-     iIntros "!> $". done.
+     iIntros "!> $".
    Qed.
 
-   Lemma imp_EArraySet2 `{Encode A} {Φ : unit → iProp Σ} {ζ}
+   Lemma imp_EArraySet2 `{Encode A, Inhabited A} {Φ : unit → iProp Σ} {ζ}
      (Φ3 : A → iProp Σ) (Φ1 : array → iProp Σ) (Φ2 : Z → iProp Σ) e1 e2 e3 :
      imp eval η e1 @ E <|Ψ|> ⟨⟨ ζ ⟩⟩ {{ λ a, Φ1 a }} -∗
      imp eval η e2 @ E <|Ψ|> ⟨⟨ ζ ⟩⟩ {{ λ i, Φ2 i }} -∗
@@ -400,72 +302,24 @@ Section array_resources.
      rewrite /continue /= bind_ret.
      iNext.
      iDestruct "P" as "((%Hle & %Hlt & Hslice) & P)".
-
      iDestruct "Harr" as "(%Hlen' & %Hbound)".
      iDestruct "Hslice" as "(%Hlen & Hslice)".
-
-     (* Decompose [ls] into [lj ++ slice ++ _]. *)
-     pose proof (cut_out_slice j (length xs) a ltac:(lia) ltac:(lia))
-       as (lj & slice & lextra & Hls & Hj & Hslice).
-     (* Turn [take _ (drop _ ls)] into [slice]. *)
-     rewrite Hj {1}Hls. drop.
-     rewrite Hslice. take.
-
-     assert (¬ (i - j < 0)) as Heqf by lia.
-
-     rewrite (signed_repr i); last representable.
-     pose proof (lookup_valid_is_Some xs (i - j) ltac:(lia)) as (x & Hlookup).
-
-     (* [Decompose [xs] intl [xk ++ x :: _]. *)
-     pose proof (list_elem_of_split_length xs (i - j) _ Hlookup)
-       as (xk & xrest & Hxs & Hxk).
-     rewrite {1}Hxs.
-
-     (* Inversions on [Hslice] gives us that
-        [slice] = [slicek ++ l :: _]. *)
-     iDestruct (big_sepL2_app_inv_r with "Hslice")
-       as "(%slicek & %slice' & -> & Hslice1 & Hslice2)".
-     iDestruct (big_sepL2_cons_inv_r with "Hslice2") as
-       "(%l & %slicerest & -> & Hl & Hslice2)".
-
-     (* We can now prove that [ls !! i] = [Some l]. *)
-     rewrite {2}Hls lookup_app_r; last lia.
-     rewrite <- Hj.
-     rewrite <- app_assoc. iPoseProof (big_sepL2_length with "Hslice1") as "%Hleneq".
-     assert (length a = j + length slicek + 1 + length slicerest + length lextra).
-     { rewrite Hls. rewrite !length_app. rewrite length_cons. lia. }
-     assert (length slicek = length xk) by (rewrite /length; lia).
-     rewrite lookup_app_r; last lia.
-     assert (i - j - length slicek = 0) as -> by lia.
-     rewrite <- app_comm_cons.
-     rewrite lookup_cons_eq_0.
+     rewrite signed_repr; last representable.
+     rewrite list_lookup_lookup_total_valid; last lia.
+     iPoseProof (big_sepLZ2_insert_seg_acc i with "Hslice")
+       as "(Hl & Hslice)"; try lia.
 
      iApply (imp_store with "Hl").
      rewrite /continue; iIntros "!> Hl /=".
      iApply imp_ret; first encode.
      iApply "P".
-     iCombine ("Hl Hslice2") as "Hslice2".
-     iPoseProof (big_sepL2_cons (λ _ l' x', pointsto l' (DfracOwn 1) (V #x')) with "Hslice2") as "Hslice2".
-     iPoseProof (big_sepL2_app with "Hslice1 Hslice2") as "Hslice".
-     iSplit.
-     { iPureIntro. rewrite length_insert. lia. }
-     assert ((xk ++ y :: xrest) = <[i-j:=y]> xs) as ->.
-     { rewrite Hxs.
-       rewrite insert_take_drop.
-       take. drop. reflexivity.
-       split; first lia.
-       rewrite !length_app length_cons /length.
-       rewrite /length in Hxk.
-       lia. }
-     rewrite {1}Hls.
-     rewrite Hj. rewrite drop_app drop_all Z.sub_diag drop_none. simpl.
-     rewrite length_insert.
-     assert (length xs = length (slicek ++ l :: slicerest)) as -> by lia.
-     rewrite take_app_length.
+     iSplit; length. { iPureIntro. apply Hlen. }
+     iSpecialize ("Hslice" with "Hl").
+     update.
      iApply "Hslice".
    Qed.
 
-   Lemma imp_EArraySet `{Encode A} {ζ}
+   Lemma imp_EArraySet `{Encode A, Inhabited A} {ζ}
      (Φ : A → iProp Σ) (i j n : Z) (a : array) xs e1 e2 e3 :
      ⌜j ≤ i⌝ -∗
      ⌜i - j < length xs⌝ -∗
